# Equation 1

![\Large T_{[m*n*p]} \to t_{i,j,k}=a_i*b_j*c_k](https://latex.codecogs.com/svg.latex?\Large%20T_{[m*n*p]}\to%20t_{i,j,k}=a_i*b_j*c_k)

# Equation 2

![\Large T_{[m*n*p]} \to t_{i,j,k}=\frac{a_i*b_j}{c_k}](https://latex.codecogs.com/svg.latex?\Large%20T_{[m*n*p]}\to%20t_{i,j,k}=\frac{a_i*b_j}{c_k})

# Equation 3

![\Large T_{[m*n*p]} \to t_{i,j,k}=A_{i,j}*b_k](https://latex.codecogs.com/svg.latex?\Large%20T_{[m*n*p]}\to%20t_{i,j,k}=A_{i,j}*b_k)

# Equation 4

![\Large T_{[m*n*p]} \to t_{i,j,k}=A_{i,j}*B_{k,i}](https://latex.codecogs.com/svg.latex?\Large%20T_{[m*n*p]}\to%20t_{i,j,k}=A_{i,j}*B_{k,i})

# Equation 5

![\Large T_{[n*n*n]}\to t_{i,j,k}=\frac{r_i}{m^2_i}*D_{i,j}*D_{i,k}*\left(-\frac{v_j}{r_j}+\frac{2}{R^2}\frac{x_i}{m_i}-\frac{v_k}{r_k}\right)](https://latex.codecogs.com/svg.latex?\Large%20T_{[n*n*n]}\to%20t_{i,j,k}=\frac{r_i}{m^2_i}*D_{i,j}*D_{i,k}*\left(-\frac{v_j}{r_j}+\frac{2}{R^2}\frac{x_i}{m_i}-\frac{v_k}{r_k}\right))
